Graph/ValueThms.thy
@@ -1,0 +1,196 @@
+section \<open>Extra Theorems for Fixed-Width Integer Words\<close>
+
+theory ValueThms
+  imports Values
+begin
+
+(* declare [[show_types=true]] *)
+
+subsubsection \<open>Support Lemmas for Upper/Lower Bounds\<close>
+
+(* these two were weirdly hard to prove given it should be by definition *)
+lemma size32: "size v = 32" for v :: "32 word"
+  using size_word.rep_eq
+  using One_nat_def add.right_neutral add_Suc_right len_of_numeral_defs(2) len_of_numeral_defs(3) mult.right_neutral mult_Suc_right numeral_2_eq_2 numeral_Bit0
+  by (smt (verit, del_insts) mult.commute)
+
+lemma size64: "size v = 64" for v :: "64 word"
+  using size_word.rep_eq
+  using One_nat_def add.right_neutral add_Suc_right len_of_numeral_defs(2) len_of_numeral_defs(3) mult.right_neutral mult_Suc_right numeral_2_eq_2 numeral_Bit0
+  by (smt (verit, del_insts) mult.commute)
+
+(* Nb. Word.sint_ge and sint_lt subsume these lemmas.
+lemma signed_int_bottom32: "-(((2::int) ^ 31)) \<le> sint (v::int32)"
+  using sint_range_size size32
+  by (smt (verit, ccfv_SIG) One_nat_def Suc_pred add_Suc add_Suc_right eval_nat_numeral(3) nat.inject numeral_2_eq_2 numeral_Bit0 numeral_Bit1 zero_less_numeral)
+
+lemma signed_int_top32: "(2 ^ 31) - 1 \<ge> sint (v::int32)"
+  using sint_range_size size32
+  by (smt (verit, ccfv_SIG) One_nat_def Suc_pred add_Suc add_Suc_right eval_nat_numeral(3) nat.inject numeral_2_eq_2 numeral_Bit0 numeral_Bit1 zero_less_numeral)
+*)
+
+lemma lower_bounds_equiv: 
+  assumes "0 < N"
+  shows "-(((2::int) ^ (N-1))) = (2::int) ^ N div 2 * - 1"
+  by (simp add: assms int_power_div_base)
+
+lemma upper_bounds_equiv:
+  assumes "0 < N"
+  shows "(2::int) ^ (N-1) = (2::int) ^ N div 2"
+  by (simp add: assms int_power_div_base)
+
+
+text \<open>Some min/max bounds for 64-bit words\<close>
+
+lemma bit_bounds_min64: "((fst (bit_bounds 64))) \<le> (sint (v::int64))"
+  unfolding bit_bounds.simps fst_def
+  using sint_ge[of v] by simp
+
+lemma bit_bounds_max64: "((snd (bit_bounds 64))) \<ge> (sint (v::int64))"
+  unfolding bit_bounds.simps fst_def
+  using sint_lt[of v] by simp
+
+
+text \<open>Extend these min/max bounds to extracting smaller signed words using $signed\_take\_bit$.\<close>
+
+text \<open>Note: we could use signed to convert between bit-widths, instead of 
+  signed\_take\_bit.  But that would have to be done separately for each bit-width type.\<close>
+
+value "sint(signed_take_bit 7 (128 :: int8))"
+
+
+ML_val \<open>@{thm signed_take_bit_decr_length_iff}\<close>
+declare [[show_types=true]]
+ML_val \<open>@{thm signed_take_bit_int_less_exp}\<close>
+
+
+lemma signed_take_bit_int_less_exp_word:
+  fixes ival :: "'a :: len word"
+  assumes "n < LENGTH('a)"
+  shows "sint(signed_take_bit n ival) < (2::int) ^ n"
+  apply transfer
+  by (smt (verit, best) not_take_bit_negative signed_take_bit_eq_take_bit_shift 
+     signed_take_bit_int_less_exp take_bit_int_greater_self_iff) 
+
+lemma signed_take_bit_int_greater_eq_minus_exp_word:
+  fixes ival :: "'a :: len word"
+  assumes "n < LENGTH('a)"
+  shows "- (2 ^ n) \<le> sint(signed_take_bit n ival)"
+  apply transfer
+  by (smt (verit, best) signed_take_bit_int_greater_eq_minus_exp 
+     signed_take_bit_int_greater_eq_self_iff signed_take_bit_int_less_exp)
+
+lemma signed_take_bit_range:
+  fixes ival :: "'a :: len word"
+  assumes "n < LENGTH('a)"
+  assumes "val = sint(signed_take_bit n ival)"
+  shows "- (2 ^ n) \<le> val \<and> val < 2 ^ n"
+  using signed_take_bit_int_greater_eq_minus_exp_word signed_take_bit_int_less_exp_word
+  using assms by blast
+
+lemma int_signed_value_range:
+  fixes ival :: "int64"
+  assumes "val = int_signed_value n ival"
+  shows "- (2 ^ (n - 1)) \<le> val \<and> val < 2 ^ (n - 1)"
+  using signed_take_bit_range assms
+  by (smt (verit, ccfv_SIG) One_nat_def diff_less int_signed_value.elims len_gt_0 len_num1 power_less_imp_less_exp power_strict_increasing sint_greater_eq sint_less)
+
+
+text \<open>Some lemmas about unsigned words smaller than 64-bit, for zero-extend operators.\<close>
+
+lemma take_bit_smaller_range:
+  fixes ival :: "'a :: len word"
+  assumes "n < LENGTH('a)"
+  assumes "val = sint(take_bit n ival)"
+  shows "0 \<le> val \<and> val < (2::int) ^ n"
+  by (simp add: assms signed_take_bit_eq)
+
+lemma take_bit_same_size_nochange:
+  fixes ival :: "'a :: len word"
+  assumes "n = LENGTH('a)"
+  shows "ival = take_bit n ival"
+  by (simp add: assms)
+
+text \<open>A simplification lemma for $new\_int$, showing that upper bits can be ignored.\<close>
+
+lemma take_bit_redundant[simp]:
+  fixes ival :: "'a :: len word"
+  assumes "0 < n"
+  assumes "n < LENGTH('a)"
+  shows "signed_take_bit (n - 1) (take_bit n ival) = signed_take_bit (n - 1) ival"
+proof -
+  have "\<not> (n \<le> n - 1)" using assms by arith
+  then have "\<And>i . signed_take_bit (n - 1) (take_bit n i) = signed_take_bit (n-1) i"
+    using signed_take_bit_take_bit by (metis (mono_tags)) 
+  then show ?thesis
+    by blast
+qed
+
+lemma take_bit_same_size_range:
+  fixes ival :: "'a :: len word"
+  assumes "n = LENGTH('a)"
+  assumes "ival2 = take_bit n ival"
+  shows "- (2 ^ n div 2) \<le> sint ival2 \<and> sint ival2 < 2 ^ n div 2"
+  using assms lower_bounds_equiv sint_ge sint_lt by auto
+
+lemma take_bit_same_bounds:
+  fixes ival :: "'a :: len word"
+  assumes "n = LENGTH('a)"
+  assumes "ival2 = take_bit n ival"
+  shows "fst (bit_bounds n) \<le> sint ival2 \<and> sint ival2 \<le> snd (bit_bounds n)"
+  unfolding bit_bounds.simps 
+  using assms take_bit_same_size_range
+  by force
+
+
+
+text \<open>Next we show that casting a word to a wider word preserves any upper/lower bounds.
+  (These lemmas may not be needed any more, since we are not using scast now?)\<close>
+
+lemma scast_max_bound:
+  assumes "sint (v :: 'a :: len word) < M"
+  assumes "LENGTH('a) < LENGTH('b)"
+  shows "sint ((scast v) :: 'b :: len word) < M"
+  unfolding Word.scast_eq Word.sint_sbintrunc'
+  using Bit_Operations.signed_take_bit_int_eq_self_iff
+  by (smt (verit, best) One_nat_def assms(1) assms(2) decr_length_less_iff linorder_not_le power_strict_increasing_iff signed_take_bit_int_less_self_iff sint_greater_eq) 
+(* helpful thms?
+  Word.scast_eq: scast (?w::?'b word) = word_of_int (sint ?w)
+  Word.sint_lt: sint (?x::?'a word) < (2::int) ^ (LENGTH(?'a) - (1::nat)
+  Word.sint_uint: sint (w::'a word) = signed_take_bit (LENGTH('a) - Suc (0::nat)) (uint w)
+  Word.sint_sbintrunc' :  sint (word_of_int (?bin::int)) = signed_take_bit (LENGTH(?'a) - (1::nat)) ?bin
+  Word.int_word_sint   - moves up, takes mod, then moves down
+  Bit_Operations.signed_take_bit_int_eq_self_iff:
+    (signed_take_bit (?n::nat) (?k::int) = ?k) = (- ((2::int) ^ ?n) \<sqsubseteq> ?k \<and> ?k < (2::int) ^ ?n)
+  Bit_Operations.signed_take_bit_int_eq_self:
+    - ((2::int) ^ (?n::nat)) \<sqsubseteq> (?k::int) \<Longrightarrow> ?k < (2::int) ^ ?n \<Longrightarrow> signed_take_bit ?n ?k = ?k
+*)
+
+lemma scast_min_bound:
+  assumes "M \<le> sint (v :: 'a :: len word)"
+  assumes "LENGTH('a) < LENGTH('b)"
+  shows "M \<le> sint ((scast v) :: 'b :: len word)"
+  unfolding Word.scast_eq Word.sint_sbintrunc'
+  using Bit_Operations.signed_take_bit_int_eq_self_iff
+  by (smt (verit) One_nat_def Suc_pred assms(1) assms(2) len_gt_0 less_Suc_eq order_less_le order_less_le_trans power_le_imp_le_exp signed_take_bit_int_greater_eq_self_iff sint_lt)
+
+lemma scast_bigger_max_bound:
+  assumes "(result :: 'b :: len word) = scast (v :: 'a :: len word)"
+  shows "sint result < 2 ^ LENGTH('a) div 2"
+  using sint_lt upper_bounds_equiv scast_max_bound
+  by (smt (verit, best) assms(1) len_gt_0 signed_scast_eq signed_take_bit_int_greater_self_iff sint_ge sint_less upper_bounds_equiv) 
+
+lemma scast_bigger_min_bound:
+  assumes "(result :: 'b :: len word) = scast (v :: 'a :: len word)"
+  shows "- (2 ^ LENGTH('a) div 2) \<le> sint result"
+  using sint_ge lower_bounds_equiv scast_min_bound
+  by (smt (verit) assms len_gt_0 nat_less_le not_less scast_max_bound)
+
+lemma scast_bigger_bit_bounds:
+  assumes "(result :: 'b :: len word) = scast (v :: 'a :: len word)"
+  shows "fst (bit_bounds (LENGTH('a))) \<le> sint result \<and> sint result \<le> snd (bit_bounds (LENGTH('a)))"
+  using assms scast_bigger_min_bound scast_bigger_max_bound
+  by auto
+
+
+end
