Proofs/StampEvalThms.thy
@@ -1,75 +1,21 @@
 subsection \<open>Evaluation Stamp Theorems\<close>
 
 theory StampEvalThms
-  imports Semantics.IRTreeEvalThms
+  imports ValueThms
+          Semantics.IRTreeEvalThms
 begin
-
-subsubsection \<open>Support Lemmas for Upper/Lower Bounds\<close>
-
-(* these two were weirdly hard to prove given it should be by definition *)
-lemma size32: "size v = 32" for v :: "32 word"
-  using size_word.rep_eq
-  using One_nat_def add.right_neutral add_Suc_right len_of_numeral_defs(2) len_of_numeral_defs(3) mult.right_neutral mult_Suc_right numeral_2_eq_2 numeral_Bit0
-  by (smt (verit, del_insts) mult.commute)
-
-lemma size64: "size v = 64" for v :: "64 word"
-  using size_word.rep_eq
-  using One_nat_def add.right_neutral add_Suc_right len_of_numeral_defs(2) len_of_numeral_defs(3) mult.right_neutral mult_Suc_right numeral_2_eq_2 numeral_Bit0
-  by (smt (verit, del_insts) mult.commute)
-
-(* Nb. sint_ge and sint_lt subsume these lemmas? *)
-lemma signed_int_bottom32: "-(((2::int) ^ 31)) \<le> sint (v::int32)"
-  using sint_range_size size32
-  by (smt (verit, ccfv_SIG) One_nat_def Suc_pred add_Suc add_Suc_right eval_nat_numeral(3) nat.inject numeral_2_eq_2 numeral_Bit0 numeral_Bit1 zero_less_numeral)
-
-lemma signed_int_top32: "(2 ^ 31) - 1 \<ge> sint (v::int32)"
-  using sint_range_size size32
-  by (smt (verit, ccfv_SIG) One_nat_def Suc_pred add_Suc add_Suc_right eval_nat_numeral(3) nat.inject numeral_2_eq_2 numeral_Bit0 numeral_Bit1 zero_less_numeral)
-
-lemma lower_bounds_equiv32: "-(((2::int) ^ 31)) = (2::int) ^ 32 div 2 * - 1"
-  by fastforce
-
-lemma upper_bounds_equiv32: "(2::int) ^ 31 = (2::int) ^ 32 div 2"
-  by simp
-
-lemma bit_bounds_min32: "((fst (bit_bounds 32))) \<le> (sint (v::int32))"
-  unfolding bit_bounds.simps fst_def using signed_int_bottom32 lower_bounds_equiv32
-  by auto
-
-lemma bit_bounds_max32: "((snd (bit_bounds 32))) \<ge> (sint (v::int32))"
-  unfolding bit_bounds.simps fst_def using signed_int_top32 upper_bounds_equiv32
-  by auto
-
-lemma signed_int_bottom64: "-(((2::int) ^ 63)) \<le> sint (v::int64)"
-  using sint_range_size size64
-  by (smt (verit, ccfv_SIG) One_nat_def Suc_pred add_Suc add_Suc_right eval_nat_numeral(3) nat.inject numeral_2_eq_2 numeral_Bit0 numeral_Bit1 zero_less_numeral)
-
-lemma signed_int_top64: "(2 ^ 63) - 1 \<ge> sint (v::int64)"
-  using sint_range_size size64
-  by (smt (verit, ccfv_SIG) One_nat_def Suc_pred add_Suc add_Suc_right eval_nat_numeral(3) nat.inject numeral_2_eq_2 numeral_Bit0 numeral_Bit1 zero_less_numeral)
-
-lemma lower_bounds_equiv64: "-(((2::int) ^ 63)) = (2::int) ^ 64 div 2 * - 1"
-  by fastforce
-
-lemma upper_bounds_equiv64: "(2::int) ^ 63 = (2::int) ^ 64 div 2"
-  by simp
-
-lemma bit_bounds_min64: "((fst (bit_bounds 64))) \<le> (sint (v::int64))"
-  unfolding bit_bounds.simps fst_def using signed_int_bottom64 lower_bounds_equiv64
-  by auto
-
-lemma bit_bounds_max64: "((snd (bit_bounds 64))) \<ge> (sint (v::int64))"
-  unfolding bit_bounds.simps fst_def using signed_int_top64 upper_bounds_equiv64
-  by auto
 
 (* TODO: these will need constraints on v to make sure it fits into 32/64 bits
 lemma unrestricted_32bit_always_valid [simp]:
-  "valid_value (IntVal 32 v) (unrestricted_stamp (IntegerStamp 32 lo hi))"
-  using valid_value.simps(1) bit_bounds_min32 bit_bounds_max32
-  using unrestricted_stamp.simps(2) by presburger
+  "valid_value (new_int 32 v) (unrestricted_stamp (IntegerStamp 32 lo hi))"
+  apply auto
+  using valid_value.simps(1) bit_bounds_min32 bit_bounds_max32 new_int.simps
+  using unrestricted_stamp.simps(2) 
+*)
 
+(* TODO:
 lemma unrestricted_64bit_always_valid [simp]:
-  "valid_value (IntVal64 v) (unrestricted_stamp (IntegerStamp 64 lo hi))"
+  "valid_value (IntVal 64 v) (unrestricted_stamp (IntegerStamp 64 lo hi))"
   using valid_value.simps(2) bit_bounds_min64 bit_bounds_max64
   using unrestricted_stamp.simps(2) by presburger
 *)
@@ -80,65 +26,6 @@ lemma unary_undef: "val = UndefVal \<Longrightarrow> unary_eval op val = UndefVa
 lemma unary_obj: "val = ObjRef x \<Longrightarrow> unary_eval op val = UndefVal"
   by (cases op; auto)
 
-
-(* MU: try to generalise the above for various bit lengths. *)
-lemma lower_bounds_equiv: 
-  assumes "N > 0"
-  shows "-(((2::int) ^ (N-1))) = (2::int) ^ N div 2 * - 1"
-  by (simp add: assms int_power_div_base)
-
-lemma upper_bounds_equiv:
-  assumes "N > 0"
-  shows "(2::int) ^ (N-1) = (2::int) ^ N div 2"
-  by (simp add: assms int_power_div_base)
-
-
-text \<open>Next we show that casting a word to a wider word preserves any upper/lower bounds.\<close>
-
-lemma scast_max_bound:
-  assumes "sint (v :: 'a :: len word) < M"
-  assumes "LENGTH('a) < LENGTH('b)"
-  shows "sint ((scast v) :: 'b :: len word) < M"
-  unfolding Word.scast_eq Word.sint_sbintrunc'
-  using Bit_Operations.signed_take_bit_int_eq_self_iff
-  by (smt (verit, best) One_nat_def assms(1) assms(2) decr_length_less_iff linorder_not_le power_strict_increasing_iff signed_take_bit_int_less_self_iff sint_greater_eq) 
-(* helpful thms?
-  Word.scast_eq: scast (?w::?'b word) = word_of_int (sint ?w)
-  Word.sint_lt: sint (?x::?'a word) < (2::int) ^ (LENGTH(?'a) - (1::nat)
-  Word.sint_uint: sint (w::'a word) = signed_take_bit (LENGTH('a) - Suc (0::nat)) (uint w)
-  Word.sint_sbintrunc' :  sint (word_of_int (?bin::int)) = signed_take_bit (LENGTH(?'a) - (1::nat)) ?bin
-  Word.int_word_sint   - moves up, takes mod, then moves down
-  Bit_Operations.signed_take_bit_int_eq_self_iff:
-    (signed_take_bit (?n::nat) (?k::int) = ?k) = (- ((2::int) ^ ?n) \<sqsubseteq> ?k \<and> ?k < (2::int) ^ ?n)
-  Bit_Operations.signed_take_bit_int_eq_self:
-    - ((2::int) ^ (?n::nat)) \<sqsubseteq> (?k::int) \<Longrightarrow> ?k < (2::int) ^ ?n \<Longrightarrow> signed_take_bit ?n ?k = ?k
-*)
-
-lemma scast_min_bound:
-  assumes "M \<le> sint (v :: 'a :: len word)"
-  assumes "LENGTH('a) < LENGTH('b)"
-  shows "M \<le> sint ((scast v) :: 'b :: len word)"
-  unfolding Word.scast_eq Word.sint_sbintrunc'
-  using Bit_Operations.signed_take_bit_int_eq_self_iff
-  by (smt (verit) One_nat_def Suc_pred assms(1) assms(2) len_gt_0 less_Suc_eq order_less_le order_less_le_trans power_le_imp_le_exp signed_take_bit_int_greater_eq_self_iff sint_lt)
-
-lemma scast_bigger_max_bound:
-  assumes "(result :: 'b :: len word) = scast (v :: 'a :: len word)"
-  shows "sint result < 2 ^ LENGTH('a) div 2"
-  using sint_lt upper_bounds_equiv scast_max_bound
-  by (smt (verit, best) assms(1) len_gt_0 signed_scast_eq signed_take_bit_int_greater_self_iff sint_ge sint_less upper_bounds_equiv) 
-
-lemma scast_bigger_min_bound:
-  assumes "(result :: 'b :: len word) = scast (v :: 'a :: len word)"
-  shows "- (2 ^ LENGTH('a) div 2) \<le> sint result"
-  using sint_ge lower_bounds_equiv scast_min_bound
-  by (smt (verit) assms len_gt_0 nat_less_le not_less scast_max_bound)
-
-lemma scast_bigger_bit_bounds:
-  assumes "(result :: 'b :: len word) = scast (v :: 'a :: len word)"
-  shows "fst (bit_bounds (LENGTH('a))) \<le> sint result \<and> sint result \<le> snd (bit_bounds (LENGTH('a)))"
-  using assms scast_bigger_min_bound scast_bigger_max_bound
-  by auto
 
 (* TODO: update to allow any bit size? 
 lemma unrestricted_stamp32_always_valid [simp]:
@@ -157,34 +44,10 @@ lemma larger_stamp32_always_valid [simp]:
   using assms by (smt (z3)  bit_bounds.simps diff_le_mono linorder_not_less lower_bounds_equiv not_numeral_le_zero numerals(1) power_increasing_iff prod.sel(1) prod.sel(2) unrestricted_stamp.simps(2) valid_value.simps(1))
 *)
 
-text \<open>Possibly helpful lemmas about $signed_take_bit$, to help with UnaryNarrow.
-  Note: we could use signed to convert between bit-widths, instead of 
-  signed\_take\_bit.  But this has to be done separately for each bit-width type.\<close>
-
-value "sint(signed_take_bit 7 (128 :: int8))"
-
-
-ML_val \<open>@{thm signed_take_bit_decr_length_iff}\<close>
-declare [[show_types=true]]
-ML_val \<open>@{thm signed_take_bit_int_less_exp}\<close>
-
-lemma signed_take_bit_int_less_exp_word:
-  assumes "n < LENGTH('a)"
-  shows "sint(signed_take_bit n (k :: 'a :: len word)) < (2::int) ^ n"
-  apply transfer
-  by (smt (verit, best) not_take_bit_negative signed_take_bit_eq_take_bit_shift 
-     signed_take_bit_int_less_exp take_bit_int_greater_self_iff) 
-
-lemma signed_take_bit_int_greater_eq_minus_exp_word:
-  assumes "n < LENGTH('a)"
-  shows "- (2 ^ n) \<le> sint(signed_take_bit n (k :: 'a :: len word))"
-  apply transfer
-  by (smt (verit, best) signed_take_bit_int_greater_eq_minus_exp 
-     signed_take_bit_int_greater_eq_self_iff signed_take_bit_int_less_exp)
-
 
 
 subsubsection \<open>Support Lemmas for Integer Stamps and Associated IntVal values\<close>
+(* TODO: these do not use eval so could go up into a StampThms.thy? *)
 
 text \<open>A valid int must have the expected number of bits.\<close>
 lemma valid_int_same_bits:
@@ -220,127 +83,88 @@ lemma valid_int_unsigned_bounds:
 text \<open>Signed ints have the usual two-complement bounds.\<close>
 lemma valid_int_signed_upper_bound:
   assumes "valid_value (IntVal b val) (IntegerStamp bits lo hi)"
-  assumes "lo < 0"
   shows "int_signed_value bits val < 2 ^ (bits - 1)"
   by (metis (mono_tags, opaque_lifting) diff_le_mono int_signed_value.simps less_imp_diff_less 
        linorder_not_le one_le_numeral order_less_le_trans power_increasing signed_take_bit_int_less_exp_word sint_lt)
 
 lemma valid_int_signed_lower_bound:
   assumes "valid_value (IntVal b val) (IntegerStamp bits lo hi)"
-  assumes "lo < 0"
   shows "-(2 ^ (bits - 1)) \<le> int_signed_value bits val"
   by (smt (verit) diff_le_self int_signed_value.simps linorder_not_less power_increasing_iff signed_take_bit_int_greater_eq_minus_exp_word sint_greater_eq)
 
-
-
-
-
-lemma take_bit_smaller_range:
-  assumes "n < LENGTH('a)"
-  assumes "val = sint(take_bit n (k :: 'a :: len word))"
-  shows "0 \<le> val \<and> val < (2::int) ^ n"
-  by (simp add: assms signed_take_bit_eq)
-
-lemma take_bit_same_size_nochange:
-  assumes "n = LENGTH('a)"
-  shows "k = take_bit n (k :: 'a :: len word)"
-  by (simp add: assms)
-
-lemma take_bit_same_size_range:
-  assumes "n = LENGTH('a)"
-  assumes "val = take_bit n (k :: 'a :: len word)"
-  shows "- (2 ^ n div 2) \<le> sint val \<and>
-          sint val < 2 ^ n div 2"
-  using assms lower_bounds_equiv sint_ge sint_lt by auto
-
-
-(* TODO: delete now zero_extend_helper is gone?
-lemma zero_extend_helper_output_range32:
-  assumes "result = zero_extend_helper inBits outBits val"
-  assumes "result = IntVal32 ival"
-  shows "outBits \<le> 32 \<and> -(2 ^ (inBits - 1)) \<le> sint ival \<and> sint ival \<le> 2 ^ (inBits - 1)"
-proof -
-  have ival: "ival = (signed_take_bit (inBits - 1) val)"
-    using assms sign_extend_helper.simps
-    by (smt (verit, ccfv_SIG) Value.distinct(1) Value.inject(1) Value.simps(14) scast_id)
-  have def: "result \<noteq> UndefVal"
-    using assms
-    by blast 
-  then have ok: "0 < inBits \<and> inBits \<le> 32 \<and>
-        inBits \<le> outBits \<and> 
-        outBits \<in> valid_int_widths \<and>
-        inBits \<in> valid_int_widths"
-    using assms sign_extend_helper_ok by blast
-  then have lo: "-(2 ^ (inBits - 1)) \<le> sint (signed_take_bit (inBits - 1) val)"
-    using signed_take_bit_int_greater_eq_minus_exp_word
-    by (smt (verit, best) diff_le_self not_less power_increasing_iff sint_below_size wsst_TYs(3))
-  have hi: "sint (signed_take_bit (inBits - 1) val) < 2 ^ (inBits - 1)"
-    using signed_take_bit_int_less_exp_word
-    by (metis diff_le_mono less_imp_diff_less linorder_not_le one_le_numeral power_increasing sint_above_size wsst_TYs(3))
-  show ?thesis 
-    unfolding bit_bounds.simps fst_def ival
-    using assms ival ok lo hi order_le_less
-    by force
+text \<open>and $bit\_bounds$ versions of the above bounds.\<close>
+lemma valid_int_signed_upper_bit_bound:
+  assumes "valid_value (IntVal b val) (IntegerStamp bits lo hi)"
+  shows "int_signed_value bits val \<le> snd (bit_bounds bits)"
+proof - 
+  have "b = bits" using assms valid_int_same_bits by blast 
+  then show ?thesis 
+    using assms by force 
 qed
-*)
 
-subsubsection \<open>Support Lemmas for integer input/output size of unary and binary operators\<close>
+lemma valid_int_signed_lower_bit_bound:
+  assumes "valid_value (IntVal b val) (IntegerStamp bits lo hi)"
+  shows " fst (bit_bounds bits) \<le> int_signed_value bits val"
+proof - 
+  have "b = bits" using assms valid_int_same_bits by blast 
+  then show ?thesis
+    using assms by force 
+qed
 
-text \<open>These help us to deduce integer sizes through expressions.  Not used yet.\<close>
 
-(*
-lemma unary_abs_io32:
-  assumes "result = unary_eval UnaryAbs val"
-  assumes "result = IntVal32 r32"
-  shows "\<exists>v32. val = IntVal32 v32"
-  by (smt (verit, best) Value.distinct(9) Value.simps(6) assms(1) assms(2) intval_abs.elims unary_eval.simps(1))
+text \<open>Valid values satisfy their stamp bounds.\<close>
 
-lemma unary_abs_io64:
-  assumes "result = unary_eval UnaryAbs val"
-  assumes "result = IntVal64 r64"
-  shows "\<exists>v64. val = IntVal64 v64"
-  by (metis Value.collapse(2) Value.collapse(3) Value.collapse(4) Value.disc(3) Value.exhaust_disc Value.simps(8) assms(1) assms(2) intval_abs.simps(1) intval_abs.simps(5) is_IntVal32_def unary_eval.simps(1) unary_obj unary_undef)
+lemma valid_int_signed_range:
+  assumes "valid_value (IntVal b val) (IntegerStamp bits lo hi)"
+  shows "lo \<le> int_signed_value bits val \<and> int_signed_value bits val \<le> hi"
+  by (metis assms valid_value.simps(1))
 
-lemma unary_neg_io32:
-  assumes "result = unary_eval UnaryNeg val"
-  assumes "result = IntVal32 r32"
-  shows "\<exists>v32. val = IntVal32 v32"
-  by (metis Value.disc(7) Value.distinct(1) assms(1) assms(2) intval_negate.elims is_IntVal64_def unary_eval.simps(2))
-
-lemma unary_neg_io64:
-  assumes "result = unary_eval UnaryNeg val"
-  assumes "result = IntVal64 r64"
-  shows "\<exists>v64. val = IntVal64 v64"
-  by (metis Value.disc(3) Value.simps(8) assms(1) assms(2) intval_negate.elims is_IntVal32_def unary_eval.simps(2))
-*)
 
 
 subsubsection \<open>Validity of UnaryAbs\<close>
 
-
 text \<open>A set of lemmas for each evaltree step.
    Questions: 
-   1. do we need separate 32/64 lemmas?  
-      Yes, I think so, because almost every operator behaves differently on each width.
-      And it makes the matching more direct, does not need is\_IntVal\_def etc.
-   2. is this top-down approach (assume the result node evaluation) best?
+   1. is this top-down approach (assume the result node evaluation) best?
       Maybe.  It seems to be the shortest/simplest trigger?
 \<close>
 
 lemma unary_abs_result:
   assumes "[m,p] \<turnstile> (UnaryExpr UnaryAbs e) \<mapsto> IntVal b v"
-  obtains ve where "([m, p] \<turnstile> e \<mapsto> IntVal b ve) \<and>
-           v = (if ve <s 0 then -ve else ve)"
-  sorry
-
+  obtains ve where "([m, p] \<turnstile> e \<mapsto> ve) \<and>
+           IntVal b v = intval_abs ve"
+  using assms by force
 
 lemma unary_abs_implies_valid_value:
-  assumes 1:"[m,p] \<turnstile> expr \<mapsto> val"
-  assumes 2:"result = unary_eval UnaryAbs val"
+  assumes 1:"[m,p] \<turnstile> e1 \<mapsto> r1"
+  assumes 2:"result = unary_eval UnaryAbs r1"
   assumes 3:"result \<noteq> UndefVal"
-  assumes 4:"valid_value val (stamp_expr expr)"
-  shows "valid_value result (stamp_expr (UnaryExpr UnaryAbs expr))"
-  sorry
+  assumes 4:"valid_value r1 (stamp_expr e1)"
+  shows "valid_value result (stamp_expr (UnaryExpr UnaryAbs e1))"
+proof -
+  have "[m,p] \<turnstile> (UnaryExpr UnaryAbs e1) \<mapsto> result"
+    using assms by blast
+  then obtain b1 v1 where r1: "IntVal b1 v1 = r1"
+    using assms by (metis intval_abs.elims unary_eval.simps(1))
+  then obtain lo1 hi1 where s1: "stamp_expr e1 = IntegerStamp b1 lo1 hi1"
+    by (smt (z3) "2" "3" "4" intval_bits.simps unary_obj valid_value.elims(2))
+  then obtain v2 where r2: "result = IntVal b1 v2"
+    using assms by (metis intval_abs.simps(1) new_int.simps r1 unary_eval.simps(1)) 
+  then have "(stamp_expr (UnaryExpr UnaryAbs e1)) = unrestricted_stamp (IntegerStamp b1 lo1 hi1)"
+    by (simp add: s1)
+  then obtain sb lo2 hi2 where s2: "(stamp_expr (UnaryExpr UnaryAbs e1)) = IntegerStamp sb lo2 hi2"
+    by (metis unrestricted_stamp.simps(2))
+  then have b2: "sb = b1"
+    by (metis Stamp.inject(1) insert_iff s1 stamp_expr.simps(1) stamp_unary.simps(1) unrestricted_stamp.simps(2))
+  then show ?thesis
+    unfolding r2 s2 valid_value.simps b2
+    using 4 r1 s1
+    sorry
+qed
+
+(* TODO: intval_abs needs to expand up to 32 bits too? 
+   Or stamp could leave size unchanged? 
+*)
 
 
 subsubsection \<open>Validity of UnaryNeg\<close>
